flesh out nat reflection, fix var indexing in fms

tests/NatGoals.v
@@ -19,15 +19,46 @@ Require Import MirrorSolve.Reflection.FM.
 
 Notation bop o l r := (TFun N.sig o (l ::: r ::: hnil)).
 Notation nlit n := (TFun N.sig (N.NLit n) hnil).
-Notation tru := (TFun N.sig (N.BLit true) hnil).
-Notation zero := (nlit 0).
 
 MetaCoq Quote Definition c_plus := @plus.
+MetaCoq Quote Definition c_times := @Nat.mul.
+MetaCoq Quote Definition c_sub := @Nat.sub.
+MetaCoq Quote Definition c_div := @Nat.div.
+MetaCoq Quote Definition c_mod := @Nat.modulo.
+MetaCoq Quote Definition c_lte := @Nat.leb.
+MetaCoq Quote Definition c_lt := @Nat.ltb.
+
+(* MetaCoq Quote Definition c_gte := @Nat.geb.
+MetaCoq Quote Definition c_gt := @Nat.gtb. *)
+
+MetaCoq Quote Definition c_tru := true.
+MetaCoq Quote Definition c_fls := false.
+MetaCoq Quote Definition c_zero := 0.
+MetaCoq Quote Definition c_succ := S.
+
+Definition term2bool (t: term) : option bool := 
+  if eq_term t c_tru then Some true
+  else if eq_term t c_fls then Some false
+  else None.
+
+Fixpoint term2nat (t: term) : option nat := 
+  if eq_term t c_zero then Some 0 
+  else 
+    match t with 
+    | tApp f [e'] => 
+      if eq_term f c_succ then 
+        match term2nat e' with 
+        | Some n' => Some (S n')
+        | _ => None
+        end
+      else 
+        None
+    | _ => None
+    end.
 
 Obligation Tactic := intros.
 Equations reflect_t2tm {c: ctx N.sig} (t: term) (r_args: list (option ({srt & N.tm c srt}))) : option ({srt & N.tm c srt}) := 
-  reflect_t2tm (tApp f _) r_args := 
-  if eq_term f c_plus then
+  reflect_t2tm (tApp f es) r_args := 
     match r_args with 
     | [Some l; Some r] => 
       let (sl, tl) := l in
@@ -35,15 +66,47 @@ Equations reflect_t2tm {c: ctx N.sig} (t: term) (r_args: list (option ({srt & N.
       match sl as sl' return (N.tm c sl' -> N.tm c sr -> option ({srt & N.tm c srt})) with
       | NS => 
         match sr as sr' return (N.tm c NS -> N.tm c sr' -> option ({srt & N.tm c srt})) with
-        | NS => fun tl' tr' => Some (existT _ _ (TFun N.sig N.Plus (tl' ::: tr' ::: hnil)))
+        | NS => fun tl' tr' => 
+          if eq_term f c_plus then 
+            Some (existT _ _ (TFun N.sig N.Plus (tl' ::: tr' ::: hnil)))
+          else if eq_term f c_times then 
+            Some (existT _ _ (TFun N.sig N.Mul (tl' ::: tr' ::: hnil)))
+          else if eq_term f c_sub then 
+            Some (existT _ _ (TFun N.sig N.Sub (tl' ::: tr' ::: hnil)))
+          else if eq_term f c_mod then 
+            Some (existT _ _ (TFun N.sig N.Mod (tl' ::: tr' ::: hnil)))
+          else if eq_term f c_div then 
+            Some (existT _ _ (TFun N.sig N.Div (tl' ::: tr' ::: hnil)))
+          else if eq_term f c_lte then 
+            Some (existT _ _ (TFun N.sig N.Lte (tl' ::: tr' ::: hnil)))
+          else if eq_term f c_lt then 
+            Some (existT _ _ (TFun N.sig N.Lt (tl' ::: tr' ::: hnil)))
+          (* else if eq_term f c_gte then 
+            Some (existT _ _ (TFun N.sig N.Gte (tl' ::: tr' ::: hnil)))
+          else if eq_term f c_gt then 
+            Some (existT _ _ (TFun N.sig N.Gt (tl' ::: tr' ::: hnil))) *)
+          else 
+            None
         | _ => fun _ _ => None
         end
       | _ => fun _ _ => None
       end tl tr
-    | _ => None
-    end
-  else 
-    None;
+    | _ => 
+      match term2nat (tApp f es) with 
+      | Some n => Some (existT _ _ (TFun N.sig (N.NLit n) hnil))
+      | None => None
+      end
+    end;
+  reflect_t2tm (tConstruct ind i x) _ := 
+    let t := (tConstruct ind i x) in 
+    match term2bool t with 
+    | Some b => Some (existT _ _ (TFun N.sig (N.BLit b) hnil))
+    | None =>
+      match term2nat t with 
+      | Some n => Some (existT _ _ (TFun N.sig (N.NLit n) hnil))
+      | None => None
+      end
+    end;
   reflect_t2tm _ _ := None.
 
 MetaCoq Quote Definition nat_ind := (nat).
@@ -75,8 +138,23 @@ Definition ind2srt (i: inductive) : option N.sorts :=
   else if eq_inductive i bool_ind' then Some N.BS
   else None.
 
-MetaCoq Quote Definition test := (forall (n: nat), n = n).
-Eval vm_compute in reflect_t2fm N.sig (@reflect_t2tm) ind2srt N.sorts_eq_dec (CEmp _) test.
+MetaCoq Quote Definition test := (forall (n: nat), true = true).
+Definition test' : (FirstOrder.fm N.sig (CEmp N.sig)).
+  set (foo := reflect_t2fm N.sig (@reflect_t2tm) ind2srt N.sorts_eq_dec (CEmp _) 0 test).
+  vm_compute in foo.
+  match goal with 
+  | _ := Some ?X |- _ => exact X
+  end.
+Defined.
+
+MetaCoq Quote Definition test_2 := (forall n m, n <> 0 -> m * m = 2 * n * n -> Nat.ltb m (2 * n) = true).
+Definition test_2' : (FirstOrder.fm N.sig (CEmp N.sig)).
+  set (foo := reflect_t2fm N.sig (@reflect_t2tm) ind2srt N.sorts_eq_dec (CEmp _) 0 test_2).
+  vm_compute in foo.
+  match goal with 
+  | _ := Some ?X |- _ => exact X
+  end.
+Defined.
 
 Declare ML Module "mirrorsolve".
 
@@ -129,3 +207,24 @@ Proof.
   end.
 Admitted.
 
+Lemma nat_square_decreasing' : 
+  interp_fm (sig := N.sig) (VEmp _ N.fm_model) test_2'.
+Proof.
+  eapply n2z_corr.
+  match goal with 
+  | |- interp_fm ?v ?f => 
+    set (v' := v);
+    set (f' := f)
+  end.
+  vm_compute in f'.
+  subst v'.
+
+  unfold n2z_func.
+  autorewrite with fmap_valu.
+  subst f'.
+
+  match goal with 
+  | |- ?G => 
+    check_interp_pos G; admit
+  end.
+Admitted.
