src/theories/Reflection/Core.v
@@ -1,5 +1,6 @@
 
 Require Export MetaCoq.Template.All.
 Require Import MetaCoq.Template.Checker.
+
 Definition eq_term (l r: term) : bool := 
   @eq_term config.default_checker_flags init_graph l r.
